WIP, not working (yet): adding singed bvoperators and extract

src/ecCircuits.ml
@@ -644,19 +644,35 @@ module BaseOps = struct
       let c2 = C.reg ~size ~name:id2.id_tag in
       {circ = BWCirc(C.umull c1 c2); inps = [BWInput(id1, size); BWInput(id2, size)]}
 
-    | Some { kind = `UDiv size } -> 
+    | Some { kind = `Div (size, false) } -> 
       let id1 = EcIdent.create (temp_symbol) in
       let id2 = EcIdent.create (temp_symbol) in
       let c1 = C.reg ~size ~name:id1.id_tag in
       let c2 = C.reg ~size ~name:id2.id_tag in
       {circ = BWCirc(C.udiv c1 c2); inps = [BWInput(id1, size); BWInput(id2, size)]}
 
-    | Some { kind = `URem size } -> 
+    | Some { kind = `Div (size, true) } -> 
+      assert false
+      (* let id1 = EcIdent.create (temp_symbol) in *)
+      (* let id2 = EcIdent.create (temp_symbol) in *)
+      (* let c1 = C.reg ~size ~name:id1.id_tag in *)
+      (* let c2 = C.reg ~size ~name:id2.id_tag in *)
+      (* {circ = BWCirc(C.udiv c1 c2); inps = [BWInput(id1, size); BWInput(id2, size)]} *)
+
+    | Some { kind = `Rem (size, false) } -> 
       let id1 = EcIdent.create (temp_symbol) in
       let id2 = EcIdent.create (temp_symbol) in
       let c1 = C.reg ~size ~name:id1.id_tag in
       let c2 = C.reg ~size ~name:id2.id_tag in
       {circ = BWCirc(C.urem c1 c2); inps = [BWInput(id1, size); BWInput(id2, size)]}
+
+    | Some { kind = `Rem (size, true) } -> 
+      assert false
+      (* let id1 = EcIdent.create (temp_symbol) in *)
+      (* let id2 = EcIdent.create (temp_symbol) in *)
+      (* let c1 = C.reg ~size ~name:id1.id_tag in *)
+      (* let c2 = C.reg ~size ~name:id2.id_tag in *)
+      (* {circ = BWCirc(C.urem c1 c2); inps = [BWInput(id1, size); BWInput(id2, size)]} *)
 
     | Some { kind = `Shl  size } -> 
       let id1 = EcIdent.create (temp_symbol) in
@@ -665,12 +681,19 @@ module BaseOps = struct
       let c2 = C.reg ~size ~name:id2.id_tag in
       {circ = BWCirc(C.shift ~side:`L ~sign:`L c1 c2); inps = [BWInput(id1, size); BWInput(id2, size)]}
 
-    | Some { kind = `Shr  size } -> 
+    | Some { kind = `Shr  (size, false) } -> 
       let id1 = EcIdent.create (temp_symbol) in
       let id2 = EcIdent.create (temp_symbol) in
       let c1 = C.reg ~size ~name:id1.id_tag in
       let c2 = C.reg ~size ~name:id2.id_tag in
       {circ = BWCirc(C.shift ~side:`R ~sign:`L c1 c2); inps = [BWInput(id1, size); BWInput(id2, size)]}
+
+    | Some { kind = `Shr  (size, true) } -> 
+      let id1 = EcIdent.create (temp_symbol) in
+      let id2 = EcIdent.create (temp_symbol) in
+      let c1 = C.reg ~size ~name:id1.id_tag in
+      let c2 = C.reg ~size ~name:id2.id_tag in
+      {circ = BWCirc(C.shift ~side:`R ~sign:`A c1 c2); inps = [BWInput(id1, size); BWInput(id2, size)]}
 
     | Some { kind = `And  size } -> 
       let id1 = EcIdent.create (temp_symbol) in
@@ -691,31 +714,60 @@ module BaseOps = struct
       let c1 = C.reg ~size ~name:id1.id_tag in
       {circ = BWCirc(C.lnot_ c1 ); inps = [BWInput(id1, size)]}
 
-    | Some { kind = `ULt size } ->
+    | Some { kind = `Lt (size, false) } ->
       let id1 = EcIdent.create temp_symbol in
       let id2 = EcIdent.create temp_symbol in
       let c1 = C.reg ~size ~name:id1.id_tag in 
       let c2 = C.reg ~size ~name:id2.id_tag in 
       { circ = BWCirc([C.ugt c2 c1]); inps=[BWInput(id1, size); BWInput(id2, size)]}
+    
+    | Some { kind = `Lt (size, true) } ->
+      let id1 = EcIdent.create temp_symbol in
+      let id2 = EcIdent.create temp_symbol in
+      let c1 = C.reg ~size ~name:id1.id_tag in 
+      let c2 = C.reg ~size ~name:id2.id_tag in 
+      { circ = BWCirc([C.sgt c2 c1]); inps=[BWInput(id1, size); BWInput(id2, size)]}
 
-    | Some { kind = `ULe size } ->
+    | Some { kind = `Le (size, false) } ->
       let id1 = EcIdent.create temp_symbol in
       let id2 = EcIdent.create temp_symbol in
       let c1 = C.reg ~size ~name:id1.id_tag in 
       let c2 = C.reg ~size ~name:id2.id_tag in 
       { circ = BWCirc([C.uge c2 c1]); inps=[BWInput(id1, size); BWInput(id2, size)]}    
 
-    | Some { kind = `ZExtend (size, ext_size) } ->
-      assert (size <= ext_size);
+    | Some { kind = `Le (size, true) } ->
+      let id1 = EcIdent.create temp_symbol in
+      let id2 = EcIdent.create temp_symbol in
+      let c1 = C.reg ~size ~name:id1.id_tag in 
+      let c2 = C.reg ~size ~name:id2.id_tag in 
+      { circ = BWCirc([C.sge c2 c1]); inps=[BWInput(id1, size); BWInput(id2, size)]}    
+
+    | Some { kind = `Extend (size, out_size, false) } ->
+      assert (size <= out_size);
       let id1 = EcIdent.create (temp_symbol) in
       let c1 = C.reg ~size ~name:id1.id_tag in
-      {circ = BWCirc(C.uextend ~size:ext_size c1); inps = [BWInput (id1, size)]}
+      {circ = BWCirc(C.uextend ~size:out_size c1); inps = [BWInput (id1, size)]}
 
-    | Some { kind = `Truncate (size, trunc_sz) } ->
-      assert (size >= trunc_sz);
+    | Some { kind = `Extend (size, out_size, true) } ->
+      assert (size <= out_size);
       let id1 = EcIdent.create (temp_symbol) in
-      let c1 = C.reg ~size:trunc_sz ~name:id1.id_tag in
+      let c1 = C.reg ~size ~name:id1.id_tag in
+      {circ = BWCirc(C.sextend ~size:out_size c1); inps = [BWInput (id1, size)]}
+
+    | Some { kind = `Truncate (size, out_sz) } ->
+      assert (size >= out_sz);
+      let id1 = EcIdent.create (temp_symbol) in
+      let c1 = C.reg ~size:out_sz ~name:id1.id_tag in
       { circ = BWCirc(c1); inps=[BWInput (id1, size)]}
+
+    | Some { kind = `Extract (size, out_sz) } ->
+      assert (size >= out_sz);
+      let id1 = EcIdent.create (temp_symbol) in
+      let c1 = C.reg ~size ~name:id1.id_tag in
+      let id2 = EcIdent.create (temp_symbol) in
+      let c2 = C.reg ~size ~name:id2.id_tag in
+      let r = C.shift ~side:`L ~sign:`L c1 c2 |> List.take out_sz in
+      { circ = BWCirc(r); inps=[BWInput (id1, size); BWInput (id2, size)]}
 
     | Some { kind = `A2B ((n, w), m)} ->
       assert (n*w = m);
